Prefix(:=<https://w3id.org/pmd/co/>)
Prefix(obo:=<http://purl.obolibrary.org/obo/>)
Prefix(owl:=<http://www.w3.org/2002/07/owl#>)
Prefix(rdf:=<http://www.w3.org/1999/02/22-rdf-syntax-ns#>)
Prefix(xml:=<http://www.w3.org/XML/1998/namespace>)
Prefix(xsd:=<http://www.w3.org/2001/XMLSchema#>)
Prefix(rdfs:=<http://www.w3.org/2000/01/rdf-schema#>)
Prefix(skos:=<http://www.w3.org/2004/02/skos/core#>)
Prefix(dcterms:=<http://purl.org/dc/terms/>)


Ontology(<https://w3id.org/pmd/co/pmdco/components/pmdco-axioms-shared.owl>
Import(<https://w3id.org/pmd/co/characterization>)
Import(<https://w3id.org/pmd/co/datatransformation>)
Import(<https://w3id.org/pmd/co/devices>)
Import(<https://w3id.org/pmd/co/logistics>)
Import(<https://w3id.org/pmd/co/manufacturing>)
Import(<https://w3id.org/pmd/co/materials>)
Import(<https://w3id.org/pmd/co/qualities>)

Declaration(Class(:PMD_0020113))
Declaration(Class(:PMD_0020114))
Declaration(Class(:PMD_0020127))
Declaration(Class(:PMD_0020130))
Declaration(Class(:PMD_0020136))
Declaration(Class(:PMD_0020137))
Declaration(Class(:PMD_0020140))
Declaration(Class(:PMD_0020147))
Declaration(ObjectProperty(:PMD_0020021))
Declaration(ObjectProperty(:PMD_0020022))
Declaration(ObjectProperty(:PMD_0020141))

############################
#   Object Properties
############################

# Object Property: :PMD_0020021 (causally influences)

AnnotationAssertion(rdfs:label :PMD_0020021 "causally influences"@en)
AnnotationAssertion(skos:definition :PMD_0020021 "An entity (that is bearer of some stimulation role) causally influences another entity (that is bearer of the stimulation target role) in a process iff  the target objects qualites (and/or realizable entities?) are altered in a manner that is significant in the given context/domain of discourse.."@en)
SubObjectPropertyOf(:PMD_0020021 :PMD_0020020)
ObjectPropertyDomain(:PMD_0020021 ObjectSomeValuesFrom(obo:BFO_0000196 :PMD_0020134))
ObjectPropertyRange(:PMD_0020021 ObjectSomeValuesFrom(obo:BFO_0000196 :PMD_0020135))

# Object Property: :PMD_0020022 (intensive bearer of)

AnnotationAssertion(rdfs:comment :PMD_0020022 "TODO: check if we should force the 'o' to be a portion of matter' through:
http://ontologydesignpatterns.org/wiki/Submissions:N-Ary_Relation_Pattern_%28OWL_2%29
or
https://www.w3.org/TR/swbp-n-aryRelations/"@en)
AnnotationAssertion(rdfs:label :PMD_0020022 "intensive bearer of"@en)
AnnotationAssertion(skos:definition :PMD_0020022 "Intensive bearer of is a chain that allows to connect objects to intensive properties through \"the matter they consist of\"."@en)
AnnotationAssertion(skos:example :PMD_0020022 "This piece of metal intensive bearer of some temperature."@en)
SubObjectPropertyOf(:PMD_0020022 owl:topObjectProperty)

# Object Property: :PMD_0020141 (integral bearer of)

AnnotationAssertion(rdfs:label :PMD_0020141 "integral bearer of"@en)
AnnotationAssertion(skos:definition :PMD_0020141 "Integral bearer of is a property chain linking an object or object aggregate O that consits of a portion of matter PM to a SDC Q that inheres in 'portions of matter' only:
O -consists of-> PM -bearer of-> Q"@en)
AnnotationAssertion(skos:example :PMD_0020141 "Talking colloquially about Intensive thermodynamic properties of an object requires this property."@en)
SubObjectPropertyOf(:PMD_0020141 obo:BFO_0000196)
ObjectPropertyDomain(:PMD_0020141 ObjectUnionOf(obo:BFO_0000027 obo:BFO_0000030))
ObjectPropertyRange(:PMD_0020141 obo:BFO_0000020)



############################
#   Classes
############################

# Class: :PMD_0000005 (Behavioral Material Property)

SubClassOf(:PMD_0000005 ObjectAllValuesFrom(obo:BFO_0000197 :PMD_0000000))

# Class: :PMD_0000852 (Metal)

SubClassOf(:PMD_0000852 ObjectIntersectionOf(:PMD_0000002 ObjectSomeValuesFrom(obo:BFO_0000178 ObjectIntersectionOf(:PMD_0020003 ObjectSomeValuesFrom(obo:BFO_0000196 :PMD_0050002)))))

# Class: :PMD_0020113 (Transfer of Energy)

AnnotationAssertion(rdfs:label :PMD_0020113 "Transfer of Energy"@en)
AnnotationAssertion(skos:definition :PMD_0020113 "Transfer of energy is a process where energy in any form is transferred from one object to another."@en)
SubClassOf(:PMD_0020113 obo:BFO_0000015)

# Class: :PMD_0020114 (Transfer of Mass)

AnnotationAssertion(rdfs:label :PMD_0020114 "Transfer of Mass"@en)
SubClassOf(:PMD_0020114 obo:BFO_0000015)

# Class: :PMD_0020127 (Transfer of Information)

AnnotationAssertion(rdfs:comment :PMD_0020127 "Transfer of information is a process where information (GDC?) is transfered from one participant to another process participant."@en)
AnnotationAssertion(rdfs:label :PMD_0020127 "Transfer of Information"@en)
AnnotationAssertion(skos:example :PMD_0020127 "The process of storing an experimental result to a database instance."@en)
SubClassOf(:PMD_0020127 obo:BFO_0000015)

# Class: :PMD_0020130 (Exchange of kinetic energy)

AnnotationAssertion(rdfs:label :PMD_0020130 "Exchange of kinetic energy"@en)
SubClassOf(:PMD_0020130 :PMD_0020113)

# Class: :PMD_0020136 (Exchange of thermal energy)

AnnotationAssertion(rdfs:label :PMD_0020136 "Exchange of thermal energy"@en)
SubClassOf(:PMD_0020136 :PMD_0020113)

# Class: :PMD_0020137 (Change of potential energy)

AnnotationAssertion(rdfs:label :PMD_0020137 "Change of potential energy"@en)
SubClassOf(:PMD_0020137 :PMD_0020113)

# Class: :PMD_0020140 (Change of elastic energy)

AnnotationAssertion(rdfs:label :PMD_0020140 "Change of elastic energy"@en)
SubClassOf(:PMD_0020140 :PMD_0020137)

# Class: :PMD_0020147 (Change of formation energy or enthalpy)

AnnotationAssertion(rdfs:label :PMD_0020147 "Change of formation energy or enthalpy"@en)
SubClassOf(:PMD_0020147 :PMD_0020113)


SubObjectPropertyOf(ObjectPropertyChain(:PMD_0020005 obo:BFO_0000196) :PMD_0020022)
)