Prefix(:=<https://w3id.org/pmd/co/>)
Prefix(owl:=<http://www.w3.org/2002/07/owl#>)
Prefix(rdf:=<http://www.w3.org/1999/02/22-rdf-syntax-ns#>)
Prefix(xml:=<http://www.w3.org/XML/1998/namespace>)
Prefix(xsd:=<http://www.w3.org/2001/XMLSchema#>)
Prefix(rdfs:=<http://www.w3.org/2000/01/rdf-schema#>)


Ontology(<https://w3id.org/pmd/co/components/pmdco-logistics.owl>
Import(<https://w3id.org/pmd/co/components/pmdco-shared.owl>)
Annotation(<http://purl.org/dc/terms/title> "Platform Material Digital Core Ontology (PMDco) - Logistics Module"@en)
Annotation(rdfs:comment "The logistics module of the PMD Core Ontology (PMDco). The scope of this module is the description of material science and engineering related logistics and general organization."@en)

Declaration(Class(:PMD_0000598))
Declaration(Class(:PMD_0000599))
Declaration(Class(:PMD_0000793))
Declaration(Class(:PMD_0000814))
Declaration(Class(:PMD_0000815))
Declaration(Class(:PMD_0000830))
Declaration(Class(:PMD_0000831))
Declaration(Class(:PMD_0000873))
Declaration(Class(:PMD_0000879))
Declaration(Class(:PMD_0000881))
Declaration(Class(:PMD_0000909))
Declaration(AnnotationProperty(<http://purl.obolibrary.org/obo/IAO_0000119>))
Declaration(AnnotationProperty(<http://purl.org/dc/terms/bibliographicCitation>))
Declaration(AnnotationProperty(<http://purl.org/dc/terms/created>))
Declaration(AnnotationProperty(<http://purl.org/dc/terms/title>))
Declaration(AnnotationProperty(<http://www.w3.org/2004/02/skos/core#definition>))



############################
#   Classes
############################

# Class: :PMD_0000014 (plan)

AnnotationAssertion(:PMD_0000060 :PMD_0000014 "true"^^xsd:boolean)

# Class: :PMD_0000598 (Abteilung)

AnnotationAssertion(rdfs:label :PMD_0000598 "Abteilung"@de)
AnnotationAssertion(rdfs:label :PMD_0000598 "department"@en)
AnnotationAssertion(<http://www.w3.org/2004/02/skos/core#definition> :PMD_0000598 "Organization that it a distinct part of an organization, typically responsible for a specific area of activity, function, or expertise, and organized under a designated leader or head to carry out its duties in alignment with the broader goals and policies of the organization."@en)
AnnotationAssertion(:PMD_0000060 :PMD_0000598 "true"^^xsd:boolean)
EquivalentClasses(:PMD_0000598 ObjectIntersectionOf(:PMD_0000879 ObjectSomeValuesFrom(<http://purl.obolibrary.org/obo/BFO_0000196> :PMD_0000599)))

# Class: :PMD_0000599 (department role)

AnnotationAssertion(rdfs:comment :PMD_0000599 "This role is also an indication that an organization is a sub section of another organization."@en)
AnnotationAssertion(rdfs:label :PMD_0000599 "department role"@en)
AnnotationAssertion(<http://www.w3.org/2004/02/skos/core#definition> :PMD_0000599 "A department role is a role describing a personal function or position within an organization that defines responsibilities or activities in a specified context."@en)
AnnotationAssertion(:PMD_0000060 :PMD_0000599 "true"^^xsd:boolean)
SubClassOf(:PMD_0000599 <http://purl.obolibrary.org/obo/BFO_0000023>)

# Class: :PMD_0000793 (initiator role)

AnnotationAssertion(rdfs:label :PMD_0000793 "initiator role"@en)
AnnotationAssertion(<http://www.w3.org/2004/02/skos/core#definition> :PMD_0000793 "An initiator role is a role describing the position or function responsible for starting or catalyzing a process, often related to material testing or experiments."@en)
SubClassOf(:PMD_0000793 <http://purl.obolibrary.org/obo/BFO_0000023>)

# Class: :PMD_0000814 (Labor)

AnnotationAssertion(<http://purl.obolibrary.org/obo/IAO_0000119> :PMD_0000814 "“Laboratory.” Merriam-Webster.com Dictionary, Merriam-Webster, https://www.merriam-webster.com/dictionary/laboratory. Accessed 24 Nov. 2022."@en)
AnnotationAssertion(rdfs:label :PMD_0000814 "Labor"@de)
AnnotationAssertion(rdfs:label :PMD_0000814 "laboratory"@en)
AnnotationAssertion(<http://www.w3.org/2004/02/skos/core#definition> :PMD_0000814 "A place equipped for experimental study in a science or for testing and analysis."@en)
AnnotationAssertion(:PMD_0000060 :PMD_0000814 "true"^^xsd:boolean)
EquivalentClasses(Annotation(:PMD_0001032 "issue: https://github.com/materialdigital/core-ontology/issues/101") :PMD_0000814 ObjectIntersectionOf(<http://purl.obolibrary.org/obo/BFO_0000029> ObjectSomeValuesFrom(<http://purl.obolibrary.org/obo/BFO_0000196> :PMD_0000815)))

# Class: :PMD_0000815 (laboratory role)

AnnotationAssertion(rdfs:label :PMD_0000815 "laboratory role"@en)
AnnotationAssertion(<http://www.w3.org/2004/02/skos/core#definition> :PMD_0000815 "A laboratory role is a role specifying the functions or activities specific to experimental and analytical tasks performed in a laboratory setting."@en)
SubClassOf(:PMD_0000815 <http://purl.obolibrary.org/obo/BFO_0000023>)

# Class: :PMD_0000830 (Hersteller)

AnnotationAssertion(rdfs:label :PMD_0000830 "Hersteller"@de)
AnnotationAssertion(rdfs:label :PMD_0000830 "manufacturer company"@en)
AnnotationAssertion(<http://www.w3.org/2004/02/skos/core#definition> :PMD_0000830 "Organization that is engaged in the industrial-scale production of goods by processing raw materials, components, or parts into finished products through the use of labor, machinery, tools, and chemical or biological processing, typically for sale to wholesalers, retailers, or directly to consumers."@en)
AnnotationAssertion(:PMD_0000060 :PMD_0000830 "true"^^xsd:boolean)
EquivalentClasses(:PMD_0000830 ObjectIntersectionOf(:PMD_0000879 ObjectSomeValuesFrom(<http://purl.obolibrary.org/obo/BFO_0000196> :PMD_0000831)))

# Class: :PMD_0000831 (manufacturer role)

AnnotationAssertion(rdfs:label :PMD_0000831 "manufacturer role"@en)
AnnotationAssertion(<http://www.w3.org/2004/02/skos/core#definition> :PMD_0000831 "The manufacturer role is a role that involves the production or fabrication of materials, components, or systems."@en)
SubClassOf(:PMD_0000831 <http://purl.obolibrary.org/obo/BFO_0000023>)

# Class: :PMD_0000873 (operator role)

AnnotationAssertion(rdfs:label :PMD_0000873 "operator role"@en)
AnnotationAssertion(<http://www.w3.org/2004/02/skos/core#definition> :PMD_0000873 "An operator role is a role indicating responsibility for operating equipment or systems, typically in a laboratory or manufacturing setting."@en)
AnnotationAssertion(:PMD_0000060 :PMD_0000873 "true"^^xsd:boolean)
SubClassOf(:PMD_0000873 <http://purl.obolibrary.org/obo/BFO_0000023>)

# Class: :PMD_0000879 (organization)

AnnotationAssertion(rdfs:label :PMD_0000879 "organization"@en)
AnnotationAssertion(<http://www.w3.org/2004/02/skos/core#definition> :PMD_0000879 "An organization is a material entity for that exists some sort of legal framework that recognises the entity and its continued existence."@en)
AnnotationAssertion(:PMD_0000060 :PMD_0000879 "true"^^xsd:boolean)
AnnotationAssertion(:PMD_0001032 :PMD_0000879 "issue: https://github.com/materialdigital/core-ontology/issues/101")
SubClassOf(:PMD_0000879 <http://purl.obolibrary.org/obo/BFO_0000040>)

# Class: :PMD_0000881 (person)

AnnotationAssertion(<http://purl.obolibrary.org/obo/IAO_0000114> :PMD_0000881 <http://purl.obolibrary.org/obo/IAO_0000123>)
AnnotationAssertion(<http://purl.obolibrary.org/obo/IAO_0000412> :PMD_0000881 "http://openenergy-platform.org/ontology/oeo/oeo-import-edits.owl"^^xsd:anyURI)
AnnotationAssertion(rdfs:label :PMD_0000881 "person"@en)
AnnotationAssertion(<http://www.w3.org/2004/02/skos/core#definition> :PMD_0000881 "A person is a human being."@en)
AnnotationAssertion(:PMD_0000060 :PMD_0000881 "true"^^xsd:boolean)
SubClassOf(Annotation(:PMD_0001032 "https://github.com/materialdigital/core-ontology/issues/102") :PMD_0000881 <http://purl.obolibrary.org/obo/BFO_0000030>)

# Class: :PMD_0000909 (Projekt)

AnnotationAssertion(rdfs:label :PMD_0000909 "Projekt"@de)
AnnotationAssertion(rdfs:label :PMD_0000909 "project"@en)
AnnotationAssertion(<http://www.w3.org/2004/02/skos/core#definition> :PMD_0000909 "A series of goal-orientated (intent) activities and interactions to achieve a specific outcome."@en)
AnnotationAssertion(<http://www.w3.org/2004/02/skos/core#definition> :PMD_0000909 "Eine Reihe von zielorientierten (absichtlichen) Aktivitäten und Interaktionen, um ein bestimmtes Ergebnis zu erzielen."@de)
AnnotationAssertion(:PMD_0000060 :PMD_0000909 "true"^^xsd:boolean)
SubClassOf(:PMD_0000909 ObjectIntersectionOf(<http://purl.obolibrary.org/obo/BFO_0000015> ObjectSomeValuesFrom(<http://purl.obolibrary.org/obo/BFO_0000055> :PMD_0000014)))


)