Prefix(:=<https://w3id.org/pmd/co/>)
Prefix(obo:=<http://purl.obolibrary.org/obo/>)
Prefix(owl:=<http://www.w3.org/2002/07/owl#>)
Prefix(rdf:=<http://www.w3.org/1999/02/22-rdf-syntax-ns#>)
Prefix(xml:=<http://www.w3.org/XML/1998/namespace>)
Prefix(xsd:=<http://www.w3.org/2001/XMLSchema#>)
Prefix(rdfs:=<http://www.w3.org/2000/01/rdf-schema#>)
Prefix(skos:=<http://www.w3.org/2004/02/skos/core#>)
Prefix(dcterms:=<http://purl.org/dc/terms/>)


Ontology(<https://w3id.org/pmd/co/pmdco/components/pmdco-axioms-shared.owl>
Import(<https://w3id.org/pmd/co/characterization>)
Import(<https://w3id.org/pmd/co/datatransformation>)
Import(<https://w3id.org/pmd/co/devices>)
Import(<https://w3id.org/pmd/co/logistics>)
Import(<https://w3id.org/pmd/co/manufacturing>)
Import(<https://w3id.org/pmd/co/materials>)
Import(<https://w3id.org/pmd/co/qualities>)

Declaration(Class(:PMD_0000548))
Declaration(Class(:PMD_0000869))
Declaration(Class(:PMD_0020113))
Declaration(Class(:PMD_0020114))
Declaration(Class(:PMD_0020127))
Declaration(Class(:PMD_0020130))
Declaration(Class(:PMD_0020136))
Declaration(Class(:PMD_0020137))
Declaration(Class(:PMD_0020140))
Declaration(Class(:PMD_0020147))
Declaration(Class(:PMD_0020185))
Declaration(Class(:PMD_0020186))
Declaration(Class(:PMD_0020187))
Declaration(Class(:PMD_0020189))
Declaration(Class(:PMD_0020190))
Declaration(Class(:PMD_0020191))
Declaration(ObjectProperty(:PMD_0020021))
Declaration(ObjectProperty(:PMD_0020022))
Declaration(ObjectProperty(:PMD_0020141))
Declaration(ObjectProperty(:PMD_0020188))

############################
#   Object Properties
############################

# Object Property: :PMD_0020021 (causally influences)

AnnotationAssertion(rdfs:label :PMD_0020021 "causally influences"@en)
AnnotationAssertion(skos:definition :PMD_0020021 "An entity (that is bearer of some stimulation role) causally influences another entity (that is bearer of the stimulation target role) in a process iff  the target objects qualites (and/or realizable entities?) are altered in a manner that is significant in the given context/domain of discourse.."@en)
SubObjectPropertyOf(:PMD_0020021 :PMD_0020020)

# Object Property: :PMD_0020022 (intensive bearer of)

AnnotationAssertion(rdfs:comment :PMD_0020022 "TODO: check if we should force the 'o' to be a portion of matter' through:
http://ontologydesignpatterns.org/wiki/Submissions:N-Ary_Relation_Pattern_%28OWL_2%29
or
https://www.w3.org/TR/swbp-n-aryRelations/"@en)
AnnotationAssertion(rdfs:label :PMD_0020022 "intensive bearer of"@en)
AnnotationAssertion(skos:definition :PMD_0020022 "Intensive bearer of is a chain that allows to connect objects to intensive properties through \"the matter they consist of\"."@en)
AnnotationAssertion(skos:example :PMD_0020022 "This piece of metal intensive bearer of some temperature."@en)
SubObjectPropertyOf(:PMD_0020022 owl:topObjectProperty)

# Object Property: :PMD_0020141 (integral bearer of)

AnnotationAssertion(rdfs:label :PMD_0020141 "integral bearer of"@en)
AnnotationAssertion(skos:definition :PMD_0020141 "Integral bearer of is a property chain linking an object or object aggregate O that consits of a portion of matter PM to a SDC Q that inheres in 'portions of matter' only:
O -consists of-> PM -bearer of-> Q"@en)
AnnotationAssertion(skos:example :PMD_0020141 "Talking colloquially about Intensive thermodynamic properties of an object requires this property."@en)
SubObjectPropertyOf(:PMD_0020141 obo:BFO_0000196)
ObjectPropertyDomain(:PMD_0020141 ObjectUnionOf(obo:BFO_0000027 obo:BFO_0000030))
ObjectPropertyRange(:PMD_0020141 obo:BFO_0000020)

# Object Property: :PMD_0020188 (refers to)

AnnotationAssertion(rdfs:label :PMD_0020188 "refers to"@en)
AnnotationAssertion(skos:definition :PMD_0020188 "The relation between a process characteristic and the SDC of a (relevant) process participant, that justifies the characterisics existance."@en)
SubObjectPropertyOf(:PMD_0020188 owl:topObjectProperty)
FunctionalObjectProperty(:PMD_0020188)
ObjectPropertyDomain(:PMD_0020188 :PMD_0020185)
ObjectPropertyRange(:PMD_0020188 obo:BFO_0000020)



############################
#   Classes
############################

# Class: :PMD_0000005 (Behavioral Material Property)

SubClassOf(:PMD_0000005 ObjectAllValuesFrom(obo:BFO_0000197 :PMD_0000000))

# Class: :PMD_0000547 (Change Of Aggregate State)

SubClassOf(:PMD_0000547 :PMD_0000548)

# Class: :PMD_0000548 (Change Of Phase)

AnnotationAssertion(rdfs:label :PMD_0000548 "Change Of Phase"@en)
AnnotationAssertion(skos:definition :PMD_0000548 "A change of phase is a process describing the transition of some participant(s) from one phase to another phase."@en)
AnnotationAssertion(skos:example :PMD_0000548 "Alpha-gamma transition when heating steel above the A1-temperature."@en)
SubClassOf(:PMD_0000548 obo:BFO_0000015)

# Class: :PMD_0000549 (Change Of Temperature)


# Class: :PMD_0000596 (Deformation)


# Class: :PMD_0000629 (Emission Of Radiation)


# Class: :PMD_0000635 (Evolution Of Damage)


# Class: :PMD_0000852 (Metal)

SubClassOf(:PMD_0000852 ObjectIntersectionOf(:PMD_0000002 ObjectSomeValuesFrom(obo:BFO_0000178 ObjectIntersectionOf(:PMD_0020003 ObjectSomeValuesFrom(obo:BFO_0000196 :PMD_0050002)))))

# Class: :PMD_0000869 (Occurence Of Chemical Reaction)

AnnotationAssertion(rdfs:label :PMD_0000869 "Occurence Of Chemical Reaction"@en)
AnnotationAssertion(skos:definition :PMD_0000869 "The occurrence of (a) chemical reaction is the process in which substances interact to form new chemical compounds or alter their molecular structure."@en)
SubClassOf(:PMD_0000869 obo:BFO_0000015)
SubClassOf(:PMD_0000869 ObjectSomeValuesFrom(obo:BFO_0000057 :PMD_0000001))

# Class: :PMD_0000870 (Occurence Of Electic Field)


# Class: :PMD_0000871 (Occurence Of Magnetic Field)


# Class: :PMD_0000882 (Phase Boundary)

SubClassOf(:PMD_0000882 ObjectSomeValuesFrom(:PMD_0001029 :PMD_0000548))

# Class: :PMD_0020113 (Transfer of Energy)

AnnotationAssertion(rdfs:label :PMD_0020113 "Transfer of Energy"@en)
AnnotationAssertion(skos:definition :PMD_0020113 "Transfer of energy is a process where energy in any form is transferred from one object to another."@en)
SubClassOf(:PMD_0020113 obo:BFO_0000015)

# Class: :PMD_0020114 (Transfer of Mass)

AnnotationAssertion(rdfs:label :PMD_0020114 "Transfer of Mass"@en)
SubClassOf(:PMD_0020114 obo:BFO_0000015)

# Class: :PMD_0020127 (Transfer of Information)

AnnotationAssertion(rdfs:comment :PMD_0020127 "Transfer of information is a process where information (GDC?) is transfered from one participant to another process participant."@en)
AnnotationAssertion(rdfs:label :PMD_0020127 "Transfer of Information"@en)
AnnotationAssertion(skos:example :PMD_0020127 "The process of storing an experimental result to a database instance."@en)
SubClassOf(:PMD_0020127 obo:BFO_0000015)

# Class: :PMD_0020130 (Exchange of kinetic energy)

AnnotationAssertion(rdfs:label :PMD_0020130 "Exchange of kinetic energy"@en)
SubClassOf(:PMD_0020130 :PMD_0020113)

# Class: :PMD_0020136 (Exchange of thermal energy)

AnnotationAssertion(rdfs:label :PMD_0020136 "Exchange of thermal energy"@en)
SubClassOf(:PMD_0020136 :PMD_0020113)

# Class: :PMD_0020137 (Change of potential energy)

AnnotationAssertion(rdfs:label :PMD_0020137 "Change of potential energy"@en)
SubClassOf(:PMD_0020137 :PMD_0020113)

# Class: :PMD_0020140 (Change of elastic energy)

AnnotationAssertion(rdfs:label :PMD_0020140 "Change of elastic energy"@en)
SubClassOf(:PMD_0020140 :PMD_0020137)

# Class: :PMD_0020147 (Change of formation energy or enthalpy)

AnnotationAssertion(rdfs:label :PMD_0020147 "Change of formation energy or enthalpy"@en)
SubClassOf(:PMD_0020147 :PMD_0020113)

# Class: :PMD_0020185 (Process characteristic)

AnnotationAssertion(rdfs:comment :PMD_0020185 "Closely related to IOF process characteristic but more explicit."@en)
AnnotationAssertion(rdfs:label :PMD_0020185 "Process characteristic"@en)
AnnotationAssertion(skos:definition :PMD_0020185 "An occurent that is characteristic to a process and one of:
1. A quantifier/GDC about time related aspects of the process (duration, moment of occurence)--> to be reviewed.
2. \"refers to\" a SDC  of an (important) process participant (e.g. the input/output participant)."@en)
SubClassOf(:PMD_0020185 obo:BFO_0000003)

# Class: :PMD_0020186 (SDC increment)

AnnotationAssertion(rdfs:label :PMD_0020186 "SDC increment"@en)
AnnotationAssertion(skos:definition :PMD_0020186 "A SDC increment represents the difference between two SDC (-values) at different points in time. It is based on the idea that the change of SDC (-value) results in the creation of a new SDC resource (IRI). (TODO: name the properties pointing to the two SDCs, e.g. initial xxx and final xxx).
A SDC increment is always bound (TODO: name binding property) to a process in which the SDC-bearer participates."@en)
AnnotationAssertion(skos:example :PMD_0020186 "The difference of the volume of an object at the start and the end of a swelling process."@en)
SubClassOf(:PMD_0020186 obo:BFO_0000020)

# Class: :PMD_0020187 (Rate)

AnnotationAssertion(rdfs:label :PMD_0020187 "Rate"@en)
AnnotationAssertion(skos:definition :PMD_0020187 "A Process characteristic that referst to a SDC increment"@en)
AnnotationAssertion(skos:definition :PMD_0020187 "The cooling rate refers to the change in temperature during the cooling process.
The production rate refers to the change in number of pieces produced.
The heart rate refers to the increment of the number of heart beats during the observation period."@en)
SubClassOf(:PMD_0020187 :PMD_0000008)

# Class: :PMD_0020189 (Transformation of energy)

AnnotationAssertion(rdfs:label :PMD_0020189 "Transformation of energy"@en)
AnnotationAssertion(skos:definition :PMD_0020189 "A process during which energy stored in some participant is transformed into another form of energy."@en)
AnnotationAssertion(skos:example :PMD_0020189 "Transformation of mechanical work to heat, transformation of potential energy to kinetic."@en)
SubClassOf(:PMD_0020189 obo:BFO_0000015)

# Class: :PMD_0020190 (Transformation of information)

AnnotationAssertion(rdfs:label :PMD_0020190 "Transformation of information"@en)
AnnotationAssertion(skos:definition :PMD_0020190 "A process during which information is transformed or altered."@en)
SubClassOf(:PMD_0020190 obo:BFO_0000015)

# Class: :PMD_0020191 (Environment)

AnnotationAssertion(rdfs:label :PMD_0020191 "Environment"@en)
AnnotationAssertion(skos:definition :PMD_0020191 "A role of an unbounded portion of matter that environs a process. The environment role indicates that its bearer is in physical contact/touching some (relevant) other process participant."@en)
SubClassOf(:PMD_0020191 obo:BFO_0000023)


DisjointClasses(:PMD_0000549 :PMD_0000596 :PMD_0000629 :PMD_0000635 :PMD_0000869 :PMD_0000870 :PMD_0000871)
DisjointClasses(:PMD_0000549 :PMD_0000596 :PMD_0000629 :PMD_0000869 :PMD_0000870 :PMD_0000871)
SubObjectPropertyOf(ObjectPropertyChain(:PMD_0020005 obo:BFO_0000196) :PMD_0020022)
)