Prefix(:=<https://w3id.org/pmd/co/>)
Prefix(owl:=<http://www.w3.org/2002/07/owl#>)
Prefix(rdf:=<http://www.w3.org/1999/02/22-rdf-syntax-ns#>)
Prefix(xml:=<http://www.w3.org/XML/1998/namespace>)
Prefix(xsd:=<http://www.w3.org/2001/XMLSchema#>)
Prefix(rdfs:=<http://www.w3.org/2000/01/rdf-schema#>)


Ontology(<https://w3id.org/pmd/co/components/pmdco-datatransformation.owl>
Import(<https://w3id.org/pmd/co/components/pmdco-shared.owl>)
Annotation(<http://purl.org/dc/terms/title> "Platform Material Digital Core Ontology (PMDco) - Data Transformation Module"@en)
Annotation(rdfs:comment "Data transformation module of the PMD Core Ontology (PMDco). The scope of this module is the description of processes and methods of transforming materials related data algorithmically, e.g. for simulations."@en)

Declaration(Class(:PMD_0000051))
Declaration(Class(:PMD_0000504))
Declaration(Class(:PMD_0000527))
Declaration(Class(:PMD_0000562))
Declaration(Class(:PMD_0000583))
Declaration(Class(:PMD_0000585))
Declaration(Class(:PMD_0000594))
Declaration(Class(:PMD_0000601))
Declaration(Class(:PMD_0000613))
Declaration(Class(:PMD_0000631))
Declaration(Class(:PMD_0000660))
Declaration(Class(:PMD_0000783))
Declaration(Class(:PMD_0000786))
Declaration(Class(:PMD_0000821))
Declaration(Class(:PMD_0000862))
Declaration(Class(:PMD_0000865))
Declaration(Class(:PMD_0000866))
Declaration(Class(:PMD_0000884))
Declaration(Class(:PMD_0000913))
Declaration(Class(:PMD_0000931))
Declaration(Class(:PMD_0000933))
Declaration(Class(:PMD_0000951))
Declaration(Class(:PMD_0000956))
Declaration(Class(:PMD_0000964))
Declaration(Class(:PMD_0001003))
Declaration(AnnotationProperty(<http://purl.org/dc/terms/bibliographicCitation>))
Declaration(AnnotationProperty(<http://purl.org/dc/terms/created>))
Declaration(AnnotationProperty(<http://purl.org/dc/terms/title>))
Declaration(AnnotationProperty(<http://www.w3.org/2004/02/skos/core#definition>))
Declaration(AnnotationProperty(<http://www.w3.org/2004/02/skos/core#example>))



############################
#   Classes
############################

# Class: :PMD_0000051 (simulation entity role)

AnnotationAssertion(rdfs:label :PMD_0000051 "simulation entity role"@en)
AnnotationAssertion(<http://www.w3.org/2004/02/skos/core#definition> :PMD_0000051 "Simulation entity role is a role that inheres in an independent continuant (IC) and is realized in a simulation process. This role enables the IC to participate in the simulation as a proxy, model, or representative of a real or hypothetical entity within the simulated context"@en)
SubClassOf(:PMD_0000051 ObjectIntersectionOf(<http://purl.obolibrary.org/obo/BFO_0000023> ObjectSomeValuesFrom(<http://purl.obolibrary.org/obo/BFO_0000054> :PMD_0000933)))
SubClassOf(:PMD_0000051 ObjectSomeValuesFrom(<http://purl.obolibrary.org/obo/RO_0000081> ObjectIntersectionOf(<http://purl.obolibrary.org/obo/BFO_0000004> ObjectSomeValuesFrom(<http://purl.obolibrary.org/obo/RO_0000056> :PMD_0000933))))

# Class: :PMD_0000504 (ab initio molecular dynamics simulation)

AnnotationAssertion(<http://purl.obolibrary.org/obo/IAO_0000114> :PMD_0000504 <http://purl.obolibrary.org/obo/IAO_0000428>)
AnnotationAssertion(<http://purl.obolibrary.org/obo/IAO_0000117> :PMD_0000504 "PMDco Team")
AnnotationAssertion(rdfs:label :PMD_0000504 "Ab Initio MD Simulation"@de)
AnnotationAssertion(rdfs:label :PMD_0000504 "ab initio molecular dynamics simulation"@en)
AnnotationAssertion(<http://www.w3.org/2004/02/skos/core#definition> :PMD_0000504 "A Simulation Process that uses quantum mechanical calculations to predict the behavior of molecular systems without empirical parameters."@en)
AnnotationAssertion(<http://www.w3.org/2004/02/skos/core#definition> :PMD_0000504 "Ein Simulationsprozess, der quantenmechanische Berechnungen verwendet, um das Verhalten molekularer Systeme ohne empirische Parameter vorherzusagen."@de)
AnnotationAssertion(<http://www.w3.org/2004/02/skos/core#example> :PMD_0000504 "Simulating the electronic structure and dynamics of a new alloy to predict its mechanical properties."@en)
SubClassOf(:PMD_0000504 :PMD_0000933)

# Class: :PMD_0000527 (Atomistische Monte Carlo Simulation)

AnnotationAssertion(<http://purl.obolibrary.org/obo/IAO_0000114> :PMD_0000527 <http://purl.obolibrary.org/obo/IAO_0000428>)
AnnotationAssertion(<http://purl.obolibrary.org/obo/IAO_0000117> :PMD_0000527 "PMDco Team")
AnnotationAssertion(rdfs:label :PMD_0000527 "Atomistische Monte Carlo Simulation"@de)
AnnotationAssertion(rdfs:label :PMD_0000527 "atomistic monte carlo simulation"@en)
AnnotationAssertion(<http://www.w3.org/2004/02/skos/core#definition> :PMD_0000527 "A Monte Carlo Simulation process that focuses on the atomic scale, where the properties and behaviors of materials are modeled by considering individual atoms and their interactions."@en)
AnnotationAssertion(<http://www.w3.org/2004/02/skos/core#definition> :PMD_0000527 "Ein Monte Carlo Simulationsprozess, der sich auf die atomare Skala konzentriert, bei dem die Eigenschaften und das Verhalten von Materialien durch die Betrachtung einzelner Atome und ihrer Wechselwirkungen modelliert werden."@de)
AnnotationAssertion(<http://www.w3.org/2004/02/skos/core#example> :PMD_0000527 "Simulating the behavior of electrons in a new alloy to predict its electrical conductivity."@en)
SubClassOf(:PMD_0000527 :PMD_0000862)

# Class: :PMD_0000562 (coarse grained simulation)

AnnotationAssertion(<http://purl.obolibrary.org/obo/IAO_0000114> :PMD_0000562 <http://purl.obolibrary.org/obo/IAO_0000428>)
AnnotationAssertion(<http://purl.obolibrary.org/obo/IAO_0000117> :PMD_0000562 "PMDco Team")
AnnotationAssertion(rdfs:label :PMD_0000562 "Coarse Grained Simulation"@de)
AnnotationAssertion(rdfs:label :PMD_0000562 "coarse grained simulation"@en)
AnnotationAssertion(<http://www.w3.org/2004/02/skos/core#definition> :PMD_0000562 "Ein Multiskalensimulation Prozess, der das System vereinfacht, indem Atome oder Moleküle zu größeren Partikeln zusammengefasst werden, wodurch die Rechenkomplexität verringert wird und die Untersuchung größerer Systeme oder längerer Zeitskalen ermöglicht wird."@de)
AnnotationAssertion(<http://www.w3.org/2004/02/skos/core#definition> :PMD_0000562 "multiscale simulation process that simplifies the system by grouping atoms or molecules into larger particles, thereby reducing computational complexity and allowing for the study of larger systems or longer time scales"@en)
AnnotationAssertion(<http://www.w3.org/2004/02/skos/core#example> :PMD_0000562 "In materials science, coarse-grained simulations are often used to study the mechanical properties of polymers. For instance, in the simulation of polymer chains, each segment of the chain might represent a group of several monomers, rather than modeling every single atom. This approach allows researchers to investigate the behavior of polymeric materials over larger scales and longer time periods, such as the viscoelastic properties of a polymer melt."@en)
SubClassOf(:PMD_0000562 :PMD_0000866)

# Class: :PMD_0000583 (Datenverarbeitung)

AnnotationAssertion(<http://purl.obolibrary.org/obo/IAO_0000114> :PMD_0000583 <http://purl.obolibrary.org/obo/IAO_0000428>)
AnnotationAssertion(<http://purl.obolibrary.org/obo/IAO_0000116> :PMD_0000583 "The subclass trees of \"Computing Process\" are currently still proposals and serve as a working basis for the discussion round with the simulation/workflow domain experts."@en)
AnnotationAssertion(<http://purl.obolibrary.org/obo/IAO_0000117> :PMD_0000583 "PMDco Team")
AnnotationAssertion(rdfs:label :PMD_0000583 "Datenverarbeitung"@de)
AnnotationAssertion(rdfs:label :PMD_0000583 "Rechenprozess"@de)
AnnotationAssertion(rdfs:label :PMD_0000583 "computing process"@en)
AnnotationAssertion(<http://www.w3.org/2004/02/skos/core#definition> :PMD_0000583 "A process that involves the systematic use of computational methods and tools to perform simulations, analyses, or data transformations to achieve specific scientific or engineering goals."@en)
AnnotationAssertion(<http://www.w3.org/2004/02/skos/core#definition> :PMD_0000583 "Ein Prozess, der die systematische Verwendung von rechnerischen Methoden und Werkzeugen umfasst, um Simulationen, Analysen oder Datenumwandlungen durchzuführen, um spezifische wissenschaftliche oder technische Ziele zu erreichen."@de)
SubClassOf(:PMD_0000583 ObjectIntersectionOf(<http://purl.obolibrary.org/obo/BFO_0000015> ObjectSomeValuesFrom(<http://purl.obolibrary.org/obo/BFO_0000055> :PMD_0000014)))

# Class: :PMD_0000585 (continuous simulation)

AnnotationAssertion(<http://purl.obolibrary.org/obo/IAO_0000114> :PMD_0000585 <http://purl.obolibrary.org/obo/IAO_0000428>)
AnnotationAssertion(rdfs:label :PMD_0000585 "continuous simulation"@en)
AnnotationAssertion(<http://www.w3.org/2004/02/skos/core#definition> :PMD_0000585 "a simulation approach where changes in a system are modeled continuously over time."@en)
AnnotationAssertion(:PMD_0000060 :PMD_0000585 "true"^^xsd:boolean)
SubClassOf(:PMD_0000585 :PMD_0000931)

# Class: :PMD_0000594 (Deep Learning)

AnnotationAssertion(<http://purl.obolibrary.org/obo/IAO_0000114> :PMD_0000594 <http://purl.obolibrary.org/obo/IAO_0000428>)
AnnotationAssertion(<http://purl.obolibrary.org/obo/IAO_0000117> :PMD_0000594 "PMDco Team")
AnnotationAssertion(<http://purl.obolibrary.org/obo/IAO_0000118> :PMD_0000594 "DL")
AnnotationAssertion(rdfs:label :PMD_0000594 "Deep Learning"@de)
AnnotationAssertion(rdfs:label :PMD_0000594 "deep learning"@en)
AnnotationAssertion(<http://www.w3.org/2004/02/skos/core#definition> :PMD_0000594 "A Simulation Process that employs artificial neural networks with many layers to model complex patterns in data."@en)
AnnotationAssertion(<http://www.w3.org/2004/02/skos/core#definition> :PMD_0000594 "Ein Simulationsprozess, der künstliche neuronale Netze mit vielen Schichten verwendet, um komplexe Muster in Daten zu modellieren."@de)
AnnotationAssertion(<http://www.w3.org/2004/02/skos/core#example> :PMD_0000594 "Using deep learning to predict the formation of defects in crystalline materials."@en)
SubClassOf(:PMD_0000594 :PMD_0000933)

# Class: :PMD_0000601 (deterministic simulation)

AnnotationAssertion(<http://purl.obolibrary.org/obo/IAO_0000114> :PMD_0000601 <http://purl.obolibrary.org/obo/IAO_0000428>)
AnnotationAssertion(rdfs:label :PMD_0000601 "deterministic simulation"@en)
AnnotationAssertion(<http://www.w3.org/2004/02/skos/core#definition> :PMD_0000601 "a simulation approach where outcomes are precisely determined through known relationships without random variability."@en)
AnnotationAssertion(:PMD_0000060 :PMD_0000601 "true"^^xsd:boolean)
SubClassOf(:PMD_0000601 :PMD_0000931)

# Class: :PMD_0000613 (discrete-event simulation)

AnnotationAssertion(<http://purl.obolibrary.org/obo/IAO_0000114> :PMD_0000613 <http://purl.obolibrary.org/obo/IAO_0000428>)
AnnotationAssertion(rdfs:label :PMD_0000613 "discrete-event simulation"@en)
AnnotationAssertion(<http://www.w3.org/2004/02/skos/core#definition> :PMD_0000613 "a simulation method where events are processed at distinct points in time, commonly used for modeling systems with discrete state changes."@en)
AnnotationAssertion(:PMD_0000060 :PMD_0000613 "true"^^xsd:boolean)
SubClassOf(:PMD_0000613 :PMD_0000931)

# Class: :PMD_0000631 (empirical potential molecular dynamics simulation)

AnnotationAssertion(<http://purl.obolibrary.org/obo/IAO_0000114> :PMD_0000631 <http://purl.obolibrary.org/obo/IAO_0000428>)
AnnotationAssertion(<http://purl.obolibrary.org/obo/IAO_0000117> :PMD_0000631 "PMDco Team")
AnnotationAssertion(rdfs:label :PMD_0000631 "Empirische Potential MD Simulation"@de)
AnnotationAssertion(rdfs:label :PMD_0000631 "empirical potential molecular dynamics simulation"@en)
AnnotationAssertion(<http://www.w3.org/2004/02/skos/core#definition> :PMD_0000631 "A Simulation Process that uses empirical potentials derived from experimental data to model the behavior of molecular systems."@en)
AnnotationAssertion(<http://www.w3.org/2004/02/skos/core#definition> :PMD_0000631 "Ein Simulationsprozess, der empirische Potentiale verwendet, die aus experimentellen Daten abgeleitet sind, um das Verhalten molekularer Systeme zu modellieren."@de)
AnnotationAssertion(<http://www.w3.org/2004/02/skos/core#example> :PMD_0000631 "Simulating the diffusion of atoms in a crystal using Lennard-Jones potentials.")
SubClassOf(:PMD_0000631 :PMD_0000933)

# Class: :PMD_0000660 (Generatives Deep Learning)

AnnotationAssertion(<http://purl.obolibrary.org/obo/IAO_0000114> :PMD_0000660 <http://purl.obolibrary.org/obo/IAO_0000428>)
AnnotationAssertion(<http://purl.obolibrary.org/obo/IAO_0000117> :PMD_0000660 "PMDco Team")
AnnotationAssertion(rdfs:label :PMD_0000660 "Generatives Deep Learning"@de)
AnnotationAssertion(rdfs:label :PMD_0000660 "generative deep learning"@en)
AnnotationAssertion(<http://www.w3.org/2004/02/skos/core#definition> :PMD_0000660 "A Deep Learning process that involves creating models capable of generating new data instances that resemble the training data."@en)
AnnotationAssertion(<http://www.w3.org/2004/02/skos/core#definition> :PMD_0000660 "Ein Deep Learning-Prozess, der Modelle erstellt, die in der Lage sind, neue Dateninstanzen zu erzeugen, die den Trainingsdaten ähneln."@de)
AnnotationAssertion(<http://www.w3.org/2004/02/skos/core#example> :PMD_0000660 "Using generative adversarial networks to design new molecular structures with desired properties, such as improved conductivity or strength."@en)
SubClassOf(:PMD_0000660 :PMD_0000594)

# Class: :PMD_0000783 (Hochdurchsatzsimulation)

AnnotationAssertion(<http://purl.obolibrary.org/obo/IAO_0000114> :PMD_0000783 <http://purl.obolibrary.org/obo/IAO_0000428>)
AnnotationAssertion(<http://purl.obolibrary.org/obo/IAO_0000117> :PMD_0000783 "PMDco Team")
AnnotationAssertion(rdfs:label :PMD_0000783 "Hochdurchsatzsimulation"@de)
AnnotationAssertion(rdfs:label :PMD_0000783 "high throughput simulation"@en)
AnnotationAssertion(<http://www.w3.org/2004/02/skos/core#definition> :PMD_0000783 "A Simulation Process that performs a large number of simulations automatically to explore a wide range of conditions."@en)
AnnotationAssertion(<http://www.w3.org/2004/02/skos/core#definition> :PMD_0000783 "Ein Simulationsprozess, der eine große Anzahl von Simulationen automatisch durchführt, um eine breite Palette von Bedingungen zu erkunden."@de)
AnnotationAssertion(<http://www.w3.org/2004/02/skos/core#example> :PMD_0000783 "Screening thousands of potential material compounds to identify those with optimal properties for battery applications."@en)
SubClassOf(:PMD_0000783 :PMD_0000933)

# Class: :PMD_0000786 (hybrid simulation)

AnnotationAssertion(<http://purl.obolibrary.org/obo/IAO_0000114> :PMD_0000786 <http://purl.obolibrary.org/obo/IAO_0000428>)
AnnotationAssertion(rdfs:label :PMD_0000786 "hybrid simulation"@en)
AnnotationAssertion(<http://www.w3.org/2004/02/skos/core#definition> :PMD_0000786 "a simulation approach that combines physical and computational models to analyze material behavior."@en)
AnnotationAssertion(:PMD_0000060 :PMD_0000786 "true"^^xsd:boolean)
SubClassOf(:PMD_0000786 :PMD_0000931)

# Class: :PMD_0000821 (machine learning)

AnnotationAssertion(<http://purl.obolibrary.org/obo/IAO_0000114> :PMD_0000821 <http://purl.obolibrary.org/obo/IAO_0000428>)
AnnotationAssertion(<http://purl.obolibrary.org/obo/IAO_0000117> :PMD_0000821 "PMDco Team")
AnnotationAssertion(<http://purl.obolibrary.org/obo/IAO_0000118> :PMD_0000821 "ML")
AnnotationAssertion(rdfs:label :PMD_0000821 "Maschinelles Lernen"@de)
AnnotationAssertion(rdfs:label :PMD_0000821 "machine learning"@en)
AnnotationAssertion(<http://www.w3.org/2004/02/skos/core#definition> :PMD_0000821 "A Simulation Process that uses algorithms to enable computers to learn from and make predictions based on data."@en)
AnnotationAssertion(<http://www.w3.org/2004/02/skos/core#definition> :PMD_0000821 "Ein Simulationsprozess, der Algorithmen verwendet, um Computern das Lernen aus Daten und das Treffen von Vorhersagen zu ermöglichen."@de)
AnnotationAssertion(<http://www.w3.org/2004/02/skos/core#example> :PMD_0000821 "Predicting the mechanical properties of composite materials based on their composition."@en)
SubClassOf(:PMD_0000821 :PMD_0000933)

# Class: :PMD_0000862 (Monte Carlo Simulation)

AnnotationAssertion(<http://purl.obolibrary.org/obo/IAO_0000114> :PMD_0000862 <http://purl.obolibrary.org/obo/IAO_0000428>)
AnnotationAssertion(<http://purl.obolibrary.org/obo/IAO_0000117> :PMD_0000862 "PMDco Team")
AnnotationAssertion(rdfs:label :PMD_0000862 "Monte Carlo Simulation"@de)
AnnotationAssertion(rdfs:label :PMD_0000862 "monte carlo simulation"@en)
AnnotationAssertion(<http://www.w3.org/2004/02/skos/core#definition> :PMD_0000862 "A Simulation Process that uses random sampling to solve physical and mathematical problems."@en)
AnnotationAssertion(<http://www.w3.org/2004/02/skos/core#definition> :PMD_0000862 "Ein Simulationsprozess, der zufällige Stichproben verwendet, um physikalische und mathematische Probleme zu lösen."@de)
AnnotationAssertion(<http://www.w3.org/2004/02/skos/core#example> :PMD_0000862 "Predicting the diffusion behavior of atoms in a metal at high temperatures."@en)
SubClassOf(:PMD_0000862 :PMD_0000933)

# Class: :PMD_0000865 (multimodal deep learning)

AnnotationAssertion(<http://purl.obolibrary.org/obo/IAO_0000114> :PMD_0000865 <http://purl.obolibrary.org/obo/IAO_0000428>)
AnnotationAssertion(<http://purl.obolibrary.org/obo/IAO_0000117> :PMD_0000865 "PMDco Team")
AnnotationAssertion(rdfs:label :PMD_0000865 "Multimodales Deep Learning"@de)
AnnotationAssertion(rdfs:label :PMD_0000865 "multimodal deep learning"@en)
AnnotationAssertion(<http://www.w3.org/2004/02/skos/core#definition> :PMD_0000865 "A Deep Learning process that integrates and processes data from multiple modalities (e.g., text, images, and audio) to improve performance and gain a more comprehensive understanding."@en)
AnnotationAssertion(<http://www.w3.org/2004/02/skos/core#definition> :PMD_0000865 "Ein Deep Learning-Prozess, der Daten aus mehreren Modalitäten (z.B. Text, Bilder und Audio) integriert und verarbeitet, um die Leistung zu verbessern und ein umfassenderes Verständnis zu erlangen."@de)
AnnotationAssertion(<http://www.w3.org/2004/02/skos/core#example> :PMD_0000865 "Combining microscopy images and spectroscopic data to predict the properties of new materials more accurately."@en)
SubClassOf(:PMD_0000865 :PMD_0000594)

# Class: :PMD_0000866 (multiscale simulation)

AnnotationAssertion(<http://purl.obolibrary.org/obo/IAO_0000114> :PMD_0000866 <http://purl.obolibrary.org/obo/IAO_0000428>)
AnnotationAssertion(<http://purl.obolibrary.org/obo/IAO_0000117> :PMD_0000866 "PMDco Team")
AnnotationAssertion(rdfs:label :PMD_0000866 "Multiskalensimulation"@de)
AnnotationAssertion(rdfs:label :PMD_0000866 "multiscale simulation"@en)
AnnotationAssertion(<http://www.w3.org/2004/02/skos/core#definition> :PMD_0000866 "A Simulation Process that integrates models at different scales to study a system's behavior."@en)
AnnotationAssertion(<http://www.w3.org/2004/02/skos/core#definition> :PMD_0000866 "Ein Simulationsprozess, der Modelle auf verschiedenen Skalen integriert, um das Verhalten eines Systems zu untersuchen."@de)
AnnotationAssertion(<http://www.w3.org/2004/02/skos/core#example> :PMD_0000866 "Studying the interaction between microstructural and macroscopic properties in metallic alloys."@en)
SubClassOf(:PMD_0000866 :PMD_0000933)

# Class: :PMD_0000884 (physical simulation)

AnnotationAssertion(<http://purl.obolibrary.org/obo/IAO_0000114> :PMD_0000884 <http://purl.obolibrary.org/obo/IAO_0000428>)
AnnotationAssertion(rdfs:label :PMD_0000884 "physical simulation"@en)
AnnotationAssertion(<http://www.w3.org/2004/02/skos/core#definition> :PMD_0000884 "a simulating approach describing the use of computational or experimental methods to replicate physical behaviors or processes under defined conditions."@en)
AnnotationAssertion(:PMD_0000060 :PMD_0000884 "true"^^xsd:boolean)
SubClassOf(:PMD_0000884 :PMD_0000931)

# Class: :PMD_0000913 (Reinforcement Learning)

AnnotationAssertion(<http://purl.obolibrary.org/obo/IAO_0000114> :PMD_0000913 <http://purl.obolibrary.org/obo/IAO_0000428>)
AnnotationAssertion(<http://purl.obolibrary.org/obo/IAO_0000117> :PMD_0000913 "PMDco Team")
AnnotationAssertion(<http://purl.obolibrary.org/obo/IAO_0000118> :PMD_0000913 "RL")
AnnotationAssertion(rdfs:label :PMD_0000913 "Reinforcement Learning"@de)
AnnotationAssertion(rdfs:label :PMD_0000913 "reinforcement learning"@en)
AnnotationAssertion(<http://www.w3.org/2004/02/skos/core#definition> :PMD_0000913 "A Deep Learning process that involves training models to make sequences of decisions by rewarding desired actions and punishing undesired ones."@en)
AnnotationAssertion(<http://www.w3.org/2004/02/skos/core#definition> :PMD_0000913 "Ein Deep Learning Prozess, der Modelle darin trainiert, Abfolgen von Entscheidungen zu treffen, indem gewünschte Aktionen belohnt und unerwünschte bestraft werden."@de)
AnnotationAssertion(<http://www.w3.org/2004/02/skos/core#example> :PMD_0000913 "Using RL to optimize the process parameters in additive manufacturing (3D printing) to achieve the desired material properties and reduce defects."@en)
SubClassOf(:PMD_0000913 :PMD_0000594)

# Class: :PMD_0000931 (simulation method specification)

AnnotationAssertion(<http://purl.obolibrary.org/obo/IAO_0000114> :PMD_0000931 <http://purl.obolibrary.org/obo/IAO_0000428>)
AnnotationAssertion(rdfs:label :PMD_0000931 "simulation method specification"@en)
AnnotationAssertion(<http://www.w3.org/2004/02/skos/core#definition> :PMD_0000931 "A plan specification that specifies the method of creating a computational or physical model to replicate the behavior of a material or system under specific conditions."@en)
AnnotationAssertion(:PMD_0000060 :PMD_0000931 "true"^^xsd:boolean)
SubClassOf(:PMD_0000931 <http://purl.obolibrary.org/obo/IAO_0000104>)

# Class: :PMD_0000933 (Simulationsprozess)

AnnotationAssertion(<http://purl.obolibrary.org/obo/IAO_0000114> :PMD_0000933 <http://purl.obolibrary.org/obo/IAO_0000428>)
AnnotationAssertion(<http://purl.obolibrary.org/obo/IAO_0000117> :PMD_0000933 "PMDco Team")
AnnotationAssertion(rdfs:label :PMD_0000933 "Simulationsprozess"@de)
AnnotationAssertion(rdfs:label :PMD_0000933 "simulation process"@en)
AnnotationAssertion(<http://www.w3.org/2004/02/skos/core#definition> :PMD_0000933 "A Computing Process that models the behavior of a system over time using mathematical or computational techniques."@en)
AnnotationAssertion(<http://www.w3.org/2004/02/skos/core#definition> :PMD_0000933 "Ein Datenverarbeitungsprozess, der das Verhalten eines Systems im Laufe der Zeit mit mathematischen oder rechnerischen Techniken modelliert"@de)
SubClassOf(:PMD_0000933 :PMD_0000583)

# Class: :PMD_0000951 (stochastic simulation)

AnnotationAssertion(<http://purl.obolibrary.org/obo/IAO_0000114> :PMD_0000951 <http://purl.obolibrary.org/obo/IAO_0000428>)
AnnotationAssertion(rdfs:label :PMD_0000951 "stochastic simulation"@en)
AnnotationAssertion(<http://www.w3.org/2004/02/skos/core#definition> :PMD_0000951 "a simulation approach that incorporates random variables to model probabilistic systems or processes."@en)
AnnotationAssertion(:PMD_0000060 :PMD_0000951 "true"^^xsd:boolean)
SubClassOf(:PMD_0000951 :PMD_0000931)

# Class: :PMD_0000956 (structural optimization simulation)

AnnotationAssertion(<http://purl.obolibrary.org/obo/IAO_0000114> :PMD_0000956 <http://purl.obolibrary.org/obo/IAO_0000428>)
AnnotationAssertion(<http://purl.obolibrary.org/obo/IAO_0000117> :PMD_0000956 "PMDco Team")
AnnotationAssertion(rdfs:label :PMD_0000956 "Strukturoptimierungssimulation"@de)
AnnotationAssertion(rdfs:label :PMD_0000956 "structural optimization simulation"@en)
AnnotationAssertion(<http://www.w3.org/2004/02/skos/core#definition> :PMD_0000956 "A Simulation Process that aims to find the most stable structure of a molecular system by minimizing its energy."@en)
AnnotationAssertion(<http://www.w3.org/2004/02/skos/core#definition> :PMD_0000956 "Ein Simulationsprozess, der darauf abzielt, die stabilste Struktur eines molekularen Systems durch Minimierung seiner Energie zu finden."@de)
AnnotationAssertion(<http://www.w3.org/2004/02/skos/core#example> :PMD_0000956 "Optimizing the atomic structure of a catalyst to enhance its performance."@en)
SubClassOf(:PMD_0000956 :PMD_0000933)

# Class: :PMD_0000964 (supervised machine learning)

AnnotationAssertion(<http://purl.obolibrary.org/obo/IAO_0000114> :PMD_0000964 <http://purl.obolibrary.org/obo/IAO_0000428>)
AnnotationAssertion(<http://purl.obolibrary.org/obo/IAO_0000117> :PMD_0000964 "PMDco Team")
AnnotationAssertion(rdfs:label :PMD_0000964 "supervised learning"@de)
AnnotationAssertion(rdfs:label :PMD_0000964 "supervised machine learning")
AnnotationAssertion(<http://www.w3.org/2004/02/skos/core#definition> :PMD_0000964 "A Machine Learning process that learns a function mapping from input data to labeled output data."@en)
AnnotationAssertion(<http://www.w3.org/2004/02/skos/core#definition> :PMD_0000964 "Ein Maschinelles Lernen Prozess, der eine Funktion erlernt, die Eingabedaten auf beschriftete Ausgabedaten abbildet."@de)
AnnotationAssertion(<http://www.w3.org/2004/02/skos/core#example> :PMD_0000964 "Training a model to predict the tensile strength of a material based on its composition and manufacturing process parameters. This involves using a dataset where the tensile strength is already known (labeled data) to train the model."@en)
SubClassOf(:PMD_0000964 :PMD_0000821)

# Class: :PMD_0001003 (unsupervised machine learning)

AnnotationAssertion(<http://purl.obolibrary.org/obo/IAO_0000114> :PMD_0001003 <http://purl.obolibrary.org/obo/IAO_0000428>)
AnnotationAssertion(<http://purl.obolibrary.org/obo/IAO_0000117> :PMD_0001003 "PMDco Team")
AnnotationAssertion(rdfs:label :PMD_0001003 "Unsupervised Learning"@de)
AnnotationAssertion(rdfs:label :PMD_0001003 "unsupervised machine learning"@en)
AnnotationAssertion(<http://www.w3.org/2004/02/skos/core#definition> :PMD_0001003 "A Machine Learning process that identifies patterns and relationships in data without using labeled outcomes."@en)
AnnotationAssertion(<http://www.w3.org/2004/02/skos/core#definition> :PMD_0001003 "Ein Maschinelles Lernen Prozess, der Muster und Zusammenhänge in Daten identifiziert, ohne beschriftete Ergebnisse zu verwenden."@de)
AnnotationAssertion(<http://www.w3.org/2004/02/skos/core#example> :PMD_0001003 "Using clustering algorithms to group similar materials based on their properties (e.g., hardness, elasticity, thermal conductivity) without prior knowledge of the categories. For instance, discovering new categories of alloy compositions that exhibit similar thermal properties."@en)
SubClassOf(:PMD_0001003 :PMD_0000821)


)